src/Examples/Sign/CallString/Example_Sign_DG_CallString_K2.thy
@@ -355,7 +355,7 @@ theorem sign_nest_2_activation_collect_sound:
   "activation_collect sign_nest_gs (admiss_exact (cs_enterc 2)) [] sign_nest_cfg (cinit_stores sign_nest_gs) v ctx
      \<subseteq> \<lbrakk>sign_ctx_sg_2 (Inl (v, ctx))\<rbrakk>"
 proof (rule activation_collect_sound[where sg = sign_ctx_sg_2 and admiss = "admiss_exact (cs_enterc 2)"
-        and seedc = "[]"
+        and startc = "[]"
         and S = "cinit_stores sign_nest_gs" and g = sign_nest_cfg and gs = sign_nest_gs])
   \<comment> \<open>ENTRY_G\<close>
   text \<open>Both the local seed \<open>s0d\<close> and the global seed \<open>s0g\<close> are \<open>cinit_sign_st\<close>'s own
